rox-star-lib/src/bytes.rs
@@ -1,14 +1,18 @@
 use crate::*;
 use std::fmt::Display;
+use secret_integers::*;
 
 pub fn u8s_to_uint32s_le(bytes: &[U8]) -> Vec<U32> {
     verif_pre!(bytes.len() % 4 == 0);
     bytes
         .chunks(4)
         .map(|chunk| {
-            U32(unsafe {
+            U32::classify(unsafe {
                 std::mem::transmute::<[u8; 4], u32>([
-                    chunk[0].0, chunk[1].0, chunk[2].0, chunk[3].0,
+                    U8::declassify(chunk[0]),
+                    U8::declassify(chunk[1]),
+                    U8::declassify(chunk[2]),
+                    U8::declassify(chunk[3])
                 ]).to_le()
             })
         })
@@ -17,9 +21,9 @@ pub fn u8s_to_uint32s_le(bytes: &[U8]) -> Vec<U32> {
 
 pub fn u8s_from_uint32s_le(ints: &[U32]) -> Vec<U8> {
     ints.iter().map(|int| {
-        let U32(int) = int;
+        let int = U32::declassify(*int);
         let bytes : [u8; 4] = unsafe { std::mem::transmute::<u32, [u8;4]>(int.to_le()) };
-        let secret_bytes : Vec<U8> = bytes.iter().map(|x| U8(*x)).collect();
+        let secret_bytes : Vec<U8> = bytes.iter().map(|x| U8::classify(*x)).collect();
         secret_bytes
     }).flatten().collect()
 }
@@ -34,11 +38,11 @@ pub fn fill<F, B : Default + Clone>(len:usize, f: F) -> Vec<B> where F: Fn(usize
 }
 
 pub fn classify_u8s(v: &[u8]) -> Vec<U8> {
-    v.iter().map(|x| U8(*x)).collect()
+    v.iter().map(|x| U8::classify(*x)).collect()
 }
 
 pub fn classify_u32s(v: &[u32]) -> Vec<U32> {
-    v.iter().map(|x| U32(*x)).collect()
+    v.iter().map(|x| U32::classify(*x)).collect()
 }
 
 pub fn format_bytes<T : Display>(v: &Vec<T>) -> String {
